Loom/Test/MinimalReproducers/TestNames.lean
@@ -2,23 +2,22 @@ import Loom.Test.Velvet.Syntax
 
 method testNames (n : Nat)
   return (result : Nat)
-  ensures result = 0
+  require h_pos : n > 0
+  ensures h_eq : result = 0
+  ensures h_le : result ≤ n
   do
   let mut i : Nat := 0
   let mut j : Nat := 0
   let mut k : Nat := 0
   while' i < n
-    invariant i ≤ n
-    invariant j = 0
-    invariant k = 0
+    invariant h_bound : i ≤ n
+    invariant h_j : j = 0
+    invariant h_k : k = 0
   do
     i := i + 1
     j := j
     k := k
   return j
-
-set_option pp.letVarTypes true in
-#print testNames
 
 prove_correct testNames by
   mvcgen' simplifying_assumptions
